\documentclass[a4paper,twocolumn]{ctexart}
\usepackage{ctex}
\usepackage{amsmath}


\graphicspath{{./figures/}}
%首行缩进两字符 利用\indent \noindent进行控制
\usepackage{indentfirst}
\setlength{\parindent}{2em}

%算法包
\usepackage{caption}
\usepackage{algorithm}
\usepackage{algorithmic}

%页边距包
\usepackage{geometry}
\geometry {left=2.0cm ,right=2.0cm,top=2.5cm,bottom=2.5cm}

%枚举
\usepackage{enumerate}

%代码
\usepackage{listings}

%算法input output
\renewcommand{\algorithmicrequire}{\textbf{Input:}} % Use Input in the format of Algorithm
\renewcommand{\algorithmicensure}{\textbf{Output:}} % Use Output in the format of Algorithm
% for fig without caption: #1: width/size; #2: fig file
\newcommand{\fignocaption}[2]{
	\begin{figure}[htp]
		\centering
		\includegraphics[#1]{#2}
	\end{figure}
}
% for fig with caption: #1: width/size; #2: fig file; #3: fig caption
\newcommand{\fig}[3]{
	\begin{figure}[htp]
		\centering
		\includegraphics[#1]{#2}
		\caption[labelInTOC]{#3}
	\end{figure}
}
%数学符号
\usepackage{amssymb}
\title{Probability And Mathmatical Statistics\\Homework 10}
\author{151220131 谢旻晖}
\date{}
\begin{document}
\maketitle
\section*{3}
\noindent\textbf{矩估计}\\
\begin{align*}
EX&=\int_{0}^{+\infty}\frac{1}{\sqrt{2\pi}\sigma}e^{-\frac{(lnx-\mu)^2}{2\sigma^2}}dx\\
\text{令}t&=\frac{lnx-\mu}{\sqrt{2}\sigma}\\
EX&=\int_{-\infty}^{+\infty}\frac{1}{\sqrt{2\pi}\sigma}e^{-t^2}\sqrt{2}\sigma e^{\sqrt{2}\sigma t+\mu}dt\\
&=\frac{1}{\sqrt{\pi}}\int_{-\infty}^{+\infty}e^{-t^2+\sqrt{2}\sigma t+\mu}dt\\
&=\frac{e^{\mu+\frac{\sigma^2}{2}}}{\sqrt{\pi}}\int_{-\infty}^{+\infty}e^{-(t-\frac{\sqrt{2}}{2}\sigma)^2}dt\\
\text{令}u&=t-\frac{\sqrt{2}}{2}\sigma\\
EX&=\frac{\sqrt{\pi}e^{\mu+\frac{\sigma^2}{2}}}{\sqrt{\pi}}\int_{-\infty}^{+\infty}\frac{1}{\sqrt{\pi}}e^{-u^2}du\\
&=e^{\mu+\frac{\sigma^2}{2}}~~~~~~~~~~(\text{右边为}N(0,\frac{1}{\sqrt{2}})\text{的概率积分})\\
EX^2&=\int_{0}^{+\infty}\frac{x}{\sqrt{2\pi}\sigma}e^{-\frac{(lnx-\mu)^2}{2\sigma^2}}dx\\
\text{令}t&=\frac{lnx-\mu}{\sqrt{2}\sigma}\\
&=\int_{-\infty}^{+\infty}\frac{1}{\sqrt{\pi}}e^{2\sqrt{2}\sigma t+2\mu -t^2}dt\\
&=\int_{-\infty}^{+\infty}\frac{1}{\sqrt{\pi}}e^{-(t-\sqrt{2}\sigma)^2}e^{2\sigma^2+2\mu}dt\\
&=\frac{e^{2\sigma^2+2\mu}}{\sqrt{\pi}}\int_{-\infty}^{+\infty}e^{-(t-\sqrt{2}\sigma)^2}dt\\
&=e^{2\sigma^2+2\mu}
\end{align*}
使用样本矩代替标准矩，得
\[
\begin{cases}
	\bar{X}&=e^{\mu+\frac{\sigma^2}{2}}\\
	\frac{1}{n}\sum_{i=1}^{n} X_i^2&=e^{2\mu+2\sigma^2}
\end{cases}
\]
解得
\begin{align*}
\hat{\mu}&=\frac{4ln\bar{X}-ln\frac{\sum_{i=1}^{n}X_i^2}{n}}{2}\\
\hat{\sigma^2}&=ln\frac{\sum_{i=1}^{n}X_i^2}{n}-2ln\bar{X}
\end{align*}
\noindent\textbf{极大似然估计}\\
似然函数为
\begin{align*}
L(\mu,\sigma^2)&=\Pi_{i=1}^{n}(2\pi \sigma^2)^{-\frac{1}{2}}X_i^{-1}e^{-\frac{(lnX_i-\mu)^2}{2\sigma^2}}\\
&=(2\pi\sigma^2)^{-\frac{n}{2}}\frac{1}{\Pi_{i=1}^{n}X_i}e^{-\frac{\sum_{i=1}^{n}(lnX_i-\mu)^2}{2\sigma^2}}\\
lnL(\mu,\sigma^2)&=-\frac{n}{2}ln(2\pi\sigma^2)+ln\frac{1}{\Pi_{i=1}^{n}X_i}-\frac{\sum_{i=1}^{n}(lnX_i-\mu)^2}{2\sigma^2}
\end{align*}
\[
\begin{cases}
\frac{\partial lnL}{\partial \sigma^2}&=-\frac{n}{2}\frac{2\pi}{2\pi\sigma^2}+\frac{\sum_{i=1}^{n}(lnX_i-\mu)^2}{2(\sigma^2)^2}=0~~~~~(1)\\
\frac{\partial lnL}{\partial \mu}&=-\frac{\sum_{i=1}^{n}2(\mu-lnX_i)}{2\sigma^2}=0~~~~~(2)
\end{cases}
\]
解得
\begin{align*}
\hat{\mu}&=\frac{\sum_{i=1}^{n}lnX_i}{n}\\
\hat{\sigma^2}&=\frac{\sum_{i=1}^{n}\left[lnX_i-\sum_{j=1}^{n}\frac{lnX_j}{n}\right]}{n}
\end{align*}
\section*{4}
\noindent\textbf{矩估计}\\

\noindent\textbf{极大似然估计}\\
\section*{11}
无偏估计意味着$E[.]=\sigma^2$.\\
\begin{align*}
E[.]&=c\sum_{i=1}^{n-1}E(X_{i+1}-X_i)^2\\
&=c\sum_{i=1}^{n-1}\left[D(X_{i+1}-X_i)+(E(X_{i+1}-X_i))^2\right]\\
&=c(n-1)2\sigma^2\\
&=\sigma^2\\
\therefore c&=\frac{1}{2(n-1)}
\end{align*}
\section*{12}
\begin{align*}
L(\sigma^2)&=\Pi_{i=1}^{n}\frac{1}{\sqrt{2\pi\sigma^2}}e^{-\frac{(X_i-\mu)^2}{2\sigma^2}}\\
lnL(\sigma^2)&=\sum_{i=1}^{n}-\frac{(X_i-\mu)^2}{2\sigma^2}+ln\frac{1}{\sqrt{2\pi\sigma^2}}\\
\frac{dlnL(\sigma^2)}{d\sigma^2}&=\sum_{i=1}^{n}\frac{(x-\mu)^2}{2\sigma^4}+\sqrt{2\pi \sigma^2}(-\frac{1}{2\pi\sigma^2})\frac{\sqrt{2\pi}}{2\sqrt{\sigma^2}}\\
&=\sum_{i=1}^{n}\frac{(x-\mu)^2}{2\sigma^4}-\frac{1}{2\sigma^2}\\
&\text{令}\frac{dlnL(\sigma^2)}{d\sigma^2}=0\\
&\frac{\sum_{i=1}^{n}(X_i-\mu)}{2\sigma^2}=\frac{n}{2\sigma^2}\\
\hat{\sigma^2}&=\frac{1}{n}\sum_{i=1}^{n}(X_i-\mu)^2
\end{align*}
\section*{13}
\section*{14}
\section*{18}
\end{document}